Wrote "program" command

Demo_Hoare.thy
@@ -2,6 +2,10 @@ theory Demo_Hoare
   imports Forward_Hoare
 begin
 
+type_synonym var = String.literal
+type_synonym mem = \<open>var \<Rightarrow> int\<close>
+datatype instruction = Add var var | Set var int | Guess var
+type_synonym "program" = "instruction list"
 
 ML \<open>
 datatype instruction = Add of var*var | Set of var*int | Guess of var
@@ -9,6 +13,14 @@ datatype instruction = Add of var*var | Set of var*int | Guess of var
     | instruction_to_term (Guess x) = \<^const>\<open>Guess\<close> $ HOLogic.mk_literal x
     | instruction_to_term (Add (x,y)) = \<^const>\<open>Add\<close> $ HOLogic.mk_literal x $ HOLogic.mk_literal y
   fun program_to_term p = map instruction_to_term p |> HOLogic.mk_list \<^typ>\<open>instruction\<close>
+  fun term_to_instruction (Const (\<^const_name>\<open>Set\<close>,_) $ x $ n) =
+            Set (HOLogic.dest_literal x, snd (HOLogic.dest_number n))
+    | term_to_instruction (Const (\<^const_name>\<open>Guess\<close>,_) $ x) =
+            Guess (HOLogic.dest_literal x)
+    | term_to_instruction (Const (\<^const_name>\<open>Add\<close>,_) $ x $ y) =
+            Add (HOLogic.dest_literal x, HOLogic.dest_literal y)
+    | term_to_instruction t = raise TERM("term_to_instruction",[t])
+  fun term_to_program t = HOLogic.dest_list t |> map term_to_instruction
 \<close>
 
 fun semantics1 :: "instruction \<Rightarrow> mem \<Rightarrow> mem set" where
@@ -33,7 +45,11 @@ structure Demo_Hoare_Logic = Hoare_Logic(
 
   val binding = \<^binding>\<open>demo_logic\<close>
 
-  fun read_program ctxt str = error "read_program"
+  fun read_program ctxt str = let
+    val t = Syntax.read_term ctxt str
+    val p = term_to_program t
+  in p end
+    
   fun read_range ctxt str = error "read_range"
 
   fun hoare_thm ctxt pre prog post = \<^const>\<open>hoare\<close> $ pre $ prog $ post |> HOLogic.mk_Trueprop
